strings for atomic propositions in HOL

hol/fitchMetaScript.sml
@@ -6,27 +6,27 @@ val _ = new_theory "fitchMeta";
 
 (* key semantic definitions *)
 
-Definition prop_of:
- (prop_of (prop_p b) = b) /\
- (prop_of (prop_neg p) = ~(prop_of p)) /\
- (prop_of (prop_and p1 p2) = ((prop_of p1) /\ (prop_of p2))) /\
- (prop_of (prop_or p1 p2) = ((prop_of p1) \/ (prop_of p2))) /\
- (prop_of (prop_imp p1 p2) = ((prop_of p1) ==> (prop_of p2))) /\
- (prop_of prop_cont = F)
+Definition prop_sem:
+ (prop_sem (prop_p x) a = a x) /\
+ (prop_sem (prop_neg p) a = ~(prop_sem p a)) /\
+ (prop_sem (prop_and p1 p2) a = ((prop_sem p1 a) /\ (prop_sem p2 a))) /\
+ (prop_sem (prop_or p1 p2) a = ((prop_sem p1 a) \/ (prop_sem p2 a))) /\
+ (prop_sem (prop_imp p1 p2) a = ((prop_sem p1 a) ==> (prop_sem p2 a))) /\
+ (prop_sem prop_cont a = F)
 End
 
 Definition premises_admitted:
- premises_admitted pl = (!p. MEM p pl ==> prop_of p)
+ premises_admitted pl a = (!p. MEM p pl ==> prop_sem p a)
 End
 
 Definition map_line_admitted:
- map_line_admitted G = (!l p. FLOOKUP G (INL l) = SOME (INL p) ==> prop_of p)
+ map_line_admitted G a = (!l p. FLOOKUP G (INL l) = SOME (INL p) ==> prop_sem p a)
 End
 
 Definition map_box_admitted:
- map_box_admitted G =
+ map_box_admitted G a =
   (!l1 l2 p1 p2. FLOOKUP G (INR (l1, l2)) = SOME (INR (p1, p2)) ==>
-  (prop_of p1 ==> prop_of p2))
+  (prop_sem p1 a ==> prop_sem p2 a))
 End
 
 (* useful induction principle *)
@@ -59,171 +59,171 @@ QED
 (* soundness of line rules *)
 
 Theorem soundness_premise:
- !G pl p l. premises_admitted pl ==>
+ !G pl p l a. premises_admitted pl a ==>
   valid_derivation G pl (derivation_deriv l p (reason_justification justification_premise)) ==>
-  prop_of p
+  prop_sem p a
 Proof
  RW_TAC list_ss [premises_admitted, valid_claim_cases]
 QED
 
 Theorem soundness_lem:
- !G pl p l. valid_derivation G pl (derivation_deriv l p (reason_justification justification_lem)) ==>
-  prop_of p
+ !G pl p l a. valid_derivation G pl (derivation_deriv l p (reason_justification justification_lem)) ==>
+  prop_sem p a
 Proof
  RW_TAC list_ss [valid_claim_cases] >>
- FULL_SIMP_TAC list_ss [prop_of]
+ FULL_SIMP_TAC list_ss [prop_sem]
 QED
 
 Theorem soundness_andi:
- !G pl p l l1 l2. map_line_admitted G ==>
+ !G pl p l l1 l2 a. map_line_admitted G a ==>
   valid_derivation G pl (derivation_deriv l p (reason_justification (justification_andi l1 l2))) ==>
-  prop_of p
+  prop_sem p a
 Proof
  RW_TAC list_ss [map_line_admitted, valid_claim_cases] >>
- FULL_SIMP_TAC list_ss [prop_of, FLOOKUP_DEF] >> METIS_TAC []
+ FULL_SIMP_TAC list_ss [prop_sem, FLOOKUP_DEF] >> METIS_TAC []
 QED
 
 Theorem soundness_copy:
- !G pl p l1 l2. map_line_admitted G ==>
+ !G pl p l1 l2 a. map_line_admitted G a ==>
   valid_derivation G pl (derivation_deriv l1 p (reason_justification (justification_copy l2))) ==>
-  prop_of p
+  prop_sem p a
 Proof
  RW_TAC list_ss [map_line_admitted, valid_claim_cases] >>
- FULL_SIMP_TAC list_ss [prop_of, FLOOKUP_DEF] >> METIS_TAC []
+ FULL_SIMP_TAC list_ss [prop_sem, FLOOKUP_DEF] >> METIS_TAC []
 QED
 
 Theorem soundness_ande1:
- !G pl p l1 l2. map_line_admitted G ==>
+ !G pl p l1 l2 a. map_line_admitted G a ==>
   valid_derivation G pl (derivation_deriv l1 p (reason_justification (justification_ande1 l2))) ==>
-  prop_of p
+  prop_sem p a
 Proof
  RW_TAC list_ss [map_line_admitted, valid_claim_cases] >>
- FULL_SIMP_TAC list_ss [prop_of, FLOOKUP_DEF] >> METIS_TAC [prop_of]
+ FULL_SIMP_TAC list_ss [prop_sem, FLOOKUP_DEF] >> METIS_TAC [prop_sem]
 QED
 
 Theorem soundness_ande2:
- !G pl p l1 l2. map_line_admitted G ==>
+ !G pl p l1 l2 a. map_line_admitted G a ==>
   valid_derivation G pl (derivation_deriv l1 p (reason_justification (justification_ande2 l2))) ==>
-  prop_of p
+  prop_sem p a
 Proof
  RW_TAC list_ss [map_line_admitted, valid_claim_cases] >>
- FULL_SIMP_TAC list_ss [prop_of, FLOOKUP_DEF] >> METIS_TAC [prop_of]
+ FULL_SIMP_TAC list_ss [prop_sem, FLOOKUP_DEF] >> METIS_TAC [prop_sem]
 QED
 
 Theorem soundness_ori1:
- !G pl p l1 l2. map_line_admitted G ==>
+ !G pl p l1 l2 a. map_line_admitted G a ==>
   valid_derivation G pl (derivation_deriv l1 p (reason_justification (justification_ori1 l2))) ==>
-  prop_of p
+  prop_sem p a
 Proof
  RW_TAC list_ss [map_line_admitted, valid_claim_cases] THEN
- FULL_SIMP_TAC list_ss [prop_of, FLOOKUP_DEF] THEN METIS_TAC []
+ FULL_SIMP_TAC list_ss [prop_sem, FLOOKUP_DEF] THEN METIS_TAC []
 QED
 
 Theorem soundness_ori2:
- !G pl p l l1 l2. map_line_admitted G ==>
+ !G pl p l l1 l2 a. map_line_admitted G a ==>
   valid_derivation G pl (derivation_deriv l1 p (reason_justification (justification_ori2 l2))) ==>
-  prop_of p
+  prop_sem p a
 Proof
  RW_TAC list_ss [map_line_admitted, valid_claim_cases] THEN
- FULL_SIMP_TAC list_ss [prop_of, FLOOKUP_DEF] THEN METIS_TAC []
+ FULL_SIMP_TAC list_ss [prop_sem, FLOOKUP_DEF] THEN METIS_TAC []
 QED
 
 Theorem soundness_impe:
- !G pl p l l1 l2. map_line_admitted G ==>
+ !G pl p l l1 l2 a. map_line_admitted G a ==>
   valid_derivation G pl (derivation_deriv l p (reason_justification (justification_impe l1 l2))) ==>
-  prop_of p
+  prop_sem p a
 Proof
  RW_TAC list_ss [map_line_admitted, valid_claim_cases] >>
- FULL_SIMP_TAC list_ss [prop_of, FLOOKUP_DEF] >> METIS_TAC [prop_of]
+ FULL_SIMP_TAC list_ss [prop_sem, FLOOKUP_DEF] >> METIS_TAC [prop_sem]
 QED
 
 Theorem soundness_nege:
- !G pl p l l1 l2. map_line_admitted G ==>
+ !G pl p l l1 l2 a. map_line_admitted G a ==>
   valid_derivation G pl (derivation_deriv l p (reason_justification (justification_nege l1 l2))) ==>
-  prop_of p
+  prop_sem p a
 Proof
  RW_TAC list_ss [map_line_admitted, valid_claim_cases] >>
- FULL_SIMP_TAC list_ss [prop_of, FLOOKUP_DEF] >> METIS_TAC [prop_of]
+ FULL_SIMP_TAC list_ss [prop_sem, FLOOKUP_DEF] >> METIS_TAC [prop_sem]
 QED
 
 Theorem soundness_conte:
- !G pl p l1 l2. map_line_admitted G ==>
+ !G pl p l1 l2 a. map_line_admitted G a ==>
   valid_derivation G pl (derivation_deriv l1 p (reason_justification (justification_conte l2))) ==>
-  prop_of p
+  prop_sem p a
 Proof
  RW_TAC list_ss [map_line_admitted, valid_claim_cases] >>
- FULL_SIMP_TAC list_ss [prop_of, FLOOKUP_DEF] >> METIS_TAC [prop_of]
+ FULL_SIMP_TAC list_ss [prop_sem, FLOOKUP_DEF] >> METIS_TAC [prop_sem]
 QED
 
 Theorem soundness_negnegi:
- !G pl p l1 l2. map_line_admitted G ==>
+ !G pl p l1 l2 a. map_line_admitted G a ==>
   valid_derivation G pl (derivation_deriv l1 p (reason_justification (justification_negnegi l2))) ==>
-  prop_of p
+  prop_sem p a
 Proof
  RW_TAC list_ss [map_line_admitted, valid_claim_cases] THEN
- FULL_SIMP_TAC list_ss [prop_of, FLOOKUP_DEF] THEN METIS_TAC []
+ FULL_SIMP_TAC list_ss [prop_sem, FLOOKUP_DEF] THEN METIS_TAC []
 QED
 
 Theorem soundness_negnege:
- !G pl p l1 l2. map_line_admitted G ==>
+ !G pl p l1 l2 a. map_line_admitted G a ==>
   valid_derivation G pl (derivation_deriv l1 p (reason_justification (justification_negnege l2))) ==>
-  prop_of p
+  prop_sem p a
 Proof
  RW_TAC list_ss [map_line_admitted, valid_claim_cases] >>
- FULL_SIMP_TAC list_ss [prop_of, FLOOKUP_DEF] >> METIS_TAC [prop_of]
+ FULL_SIMP_TAC list_ss [prop_sem, FLOOKUP_DEF] >> METIS_TAC [prop_sem]
 QED
 
 Theorem soundness_mt:
- !G pl p l l1 l2. map_line_admitted G ==>
+ !G pl p l l1 l2 a. map_line_admitted G a ==>
   valid_derivation G pl (derivation_deriv l p (reason_justification (justification_mt l1 l2))) ==>
-  prop_of p
+  prop_sem p a
 Proof
  RW_TAC list_ss [map_line_admitted, valid_claim_cases] >>
- FULL_SIMP_TAC list_ss [prop_of, FLOOKUP_DEF] >> METIS_TAC [prop_of]
+ FULL_SIMP_TAC list_ss [prop_sem, FLOOKUP_DEF] >> METIS_TAC [prop_sem]
 QED
 
 Theorem soundness_impi:
- !G pl p l l1 l2. map_box_admitted G ==>
+ !G pl p l l1 l2 a. map_box_admitted G a ==>
   valid_derivation G pl (derivation_deriv l p (reason_justification (justification_impi l1 l2))) ==>
-  prop_of p
+  prop_sem p a
 Proof
  RW_TAC list_ss [map_box_admitted, valid_claim_cases] >>
- FULL_SIMP_TAC list_ss [prop_of, FLOOKUP_DEF] >> METIS_TAC []
+ FULL_SIMP_TAC list_ss [prop_sem, FLOOKUP_DEF] >> METIS_TAC []
 QED
 
 Theorem soundness_negi:
- !G pl p l l1 l2. map_box_admitted G ==>
+ !G pl p l l1 l2 a. map_box_admitted G a ==>
   valid_derivation G pl (derivation_deriv l p (reason_justification (justification_negi l1 l2))) ==>
-  prop_of p
+  prop_sem p a
 Proof
  RW_TAC list_ss [map_box_admitted, valid_claim_cases] >>
- FULL_SIMP_TAC list_ss [prop_of, FLOOKUP_DEF] >>
- Cases_on `prop` >> METIS_TAC [prop_of]
+ FULL_SIMP_TAC list_ss [prop_sem, FLOOKUP_DEF] >>
+ Cases_on `prop` >> METIS_TAC [prop_sem]
 QED
 
 Theorem soundness_pbc:
- !G pl p l l1 l2. map_box_admitted G ==>
+ !G pl p l l1 l2 a. map_box_admitted G a ==>
   valid_derivation G pl (derivation_deriv l p (reason_justification (justification_pbc l1 l2))) ==>
-  prop_of p
+  prop_sem p a
 Proof
  RW_TAC list_ss [map_box_admitted, valid_claim_cases] >>
- FULL_SIMP_TAC list_ss [prop_of, FLOOKUP_DEF] >> METIS_TAC [prop_of]
+ FULL_SIMP_TAC list_ss [prop_sem, FLOOKUP_DEF] >> METIS_TAC [prop_sem]
 QED
 
 Theorem soundness_ore:
- !G pl p l l1 l2 l3 l4 l5. map_line_admitted G ==> map_box_admitted G ==>
+ !G pl p l l1 l2 l3 l4 l5 a. map_line_admitted G a ==> map_box_admitted G a ==>
   valid_derivation G pl (derivation_deriv l p (reason_justification (justification_ore l1 l2 l3 l4 l5))) ==>
-  prop_of p
+  prop_sem p a
 Proof
  RW_TAC list_ss [map_box_admitted, map_line_admitted, valid_claim_cases] >>
- `(prop_of prop) \/ (prop_of prop')` by METIS_TAC [prop_of, FLOOKUP_DEF] >>
- METIS_TAC [prop_of, FLOOKUP_DEF]
+ `(prop_sem prop a) \/ (prop_sem prop' a)` by METIS_TAC [prop_sem, FLOOKUP_DEF] >>
+ METIS_TAC [prop_sem, FLOOKUP_DEF]
 QED
 
 Theorem soundness_derivations:
- !G pl p l j. premises_admitted pl ==> map_line_admitted G ==> map_box_admitted G ==>
+ !G pl p l j a. premises_admitted pl a ==> map_line_admitted G a ==> map_box_admitted G a ==>
   valid_derivation G pl (derivation_deriv l p (reason_justification j)) ==>
-  prop_of p
+  prop_sem p a
 Proof
  Cases_on `j` >| [
   PROVE_TAC [soundness_premise],
@@ -250,31 +250,32 @@ QED
 (* soundness of system  *)
 
 Definition soundness_prop:
- soundness_prop (G:G) pl pr = !l j p. premises_admitted pl ==>
-  map_line_admitted G ==> map_box_admitted G ==>
+ soundness_prop (G:G) pl pr a = 
+  !l j p. premises_admitted pl a ==>
+  map_line_admitted G a ==> map_box_admitted G a ==>
   MEM (entry_derivation (derivation_deriv l p (reason_justification j))) pr ==>
-  prop_of p
+  prop_sem p a
 End
 
 Theorem soundness_empty:
- !G pl. soundness_prop G pl []
+ !G pl a. soundness_prop G pl [] a
 Proof
  RW_TAC list_ss [soundness_prop]
 QED
 
 Theorem soundness_derivation:
- !G pl l p j pr. valid_derivation G pl (derivation_deriv l p (reason_justification j)) ==>
+ !G pl l p j pr a. valid_derivation G pl (derivation_deriv l p (reason_justification j)) ==>
   valid_proof (FUPDATE G (INL l, INL p)) pl pr ==>
-  soundness_prop (FUPDATE G (INL l, INL p)) pl pr ==>
-  soundness_prop G pl (entry_derivation (derivation_deriv l p (reason_justification j)) :: pr)
+  soundness_prop (FUPDATE G (INL l, INL p)) pl pr a ==>
+  soundness_prop G pl (entry_derivation (derivation_deriv l p (reason_justification j)) :: pr) a
 Proof
  RW_TAC list_ss [soundness_prop] >- METIS_TAC [soundness_derivations] >>
- SUBGOAL_THEN ``map_line_admitted (FUPDATE (G:G) (INL l, INL p))`` ASSUME_TAC THEN RW_TAC list_ss [map_line_admitted]
+ SUBGOAL_THEN ``map_line_admitted (FUPDATE (G:G) (INL l, INL p)) a`` ASSUME_TAC THEN RW_TAC list_ss [map_line_admitted]
  >- ( Cases_on `l = l''` >> RW_TAC list_ss [map_line_admitted] >>
       FULL_SIMP_TAC list_ss [FLOOKUP_DEF, FAPPLY_FUPDATE_THM, FDOM_FUPDATE]
       >- METIS_TAC [soundness_derivations]
       >- METIS_TAC [map_line_admitted, FLOOKUP_DEF] )
- >- ( SUBGOAL_THEN ``map_box_admitted (FUPDATE (G:G) (INL l, INL p))`` ASSUME_TAC
+ >- ( SUBGOAL_THEN ``map_box_admitted (FUPDATE (G:G) (INL l, INL p)) a`` ASSUME_TAC
      >- ( FULL_SIMP_TAC list_ss [map_box_admitted, FAPPLY_FUPDATE_THM, FDOM_FUPDATE, FLOOKUP_DEF] >>
           METIS_TAC [map_box_admitted] )
      >- METIS_TAC [] )
@@ -288,19 +289,19 @@ Proof
 QED
 
 Theorem soundness_box:
- !G pl l1 l2 p1 p2 pr1 pr2 r. 
+ !G pl l1 l2 p1 p2 pr1 pr2 r a.
    LAST_DEFAULT (entry_derivation (derivation_deriv l1 p1 reason_assumption) :: pr1) entry_invalid = entry_derivation (derivation_deriv l2 p2 r) ==>
   valid_proof (FUPDATE G (INL l1, INL p1)) pl pr1 ==>
-  soundness_prop (FUPDATE G (INL l1, INL p1)) pl pr1 ==>
+  soundness_prop (FUPDATE G (INL l1, INL p1)) pl pr1 a ==>
   valid_proof (FUPDATE G (INR (l1, l2), INR (p1, p2))) pl pr2 ==>
-  soundness_prop (FUPDATE G (INR (l1, l2), INR (p1, p2))) pl pr2 ==>
-  soundness_prop G pl ((entry_box (entry_derivation (derivation_deriv l1 p1 reason_assumption) :: pr1)) :: pr2)
+  soundness_prop (FUPDATE G (INR (l1, l2), INR (p1, p2))) pl pr2 a ==>
+  soundness_prop G pl ((entry_box (entry_derivation (derivation_deriv l1 p1 reason_assumption) :: pr1)) :: pr2) a
 Proof
 RW_TAC list_ss [soundness_prop] THEN
 FULL_SIMP_TAC list_ss [] THEN
-Q.PAT_ASSUM `!l' j' p'. map_line_admitted (G |+ (INR (l1,l2),INR (p1,p2))) ==> Q` (MP_TAC o Q.SPECL [`l`, `j`, `p`]) THEN
+Q.PAT_ASSUM `!l' j' p'. map_line_admitted (G |+ (INR (l1,l2),INR (p1,p2))) a ==> Q` (MP_TAC o Q.SPECL [`l`, `j`, `p`]) THEN
 RW_TAC bool_ss [] THEN
-`map_line_admitted (G |+ (INR (l1,l2),INR (p1,p2))) /\ map_box_admitted (G |+ (INR (l1,l2),INR (p1,p2)))` suffices_by METIS_TAC [] THEN
+`map_line_admitted (G |+ (INR (l1,l2),INR (p1,p2))) a /\ map_box_admitted (G |+ (INR (l1,l2),INR (p1,p2))) a` suffices_by METIS_TAC [] THEN
 RW_TAC bool_ss [] THEN1
  (FULL_SIMP_TAC bool_ss [map_line_admitted] THEN
   RW_TAC bool_ss [FLOOKUP_DEF] THEN
@@ -328,7 +329,7 @@ Cases_on `(l1',l2') <> (l1,l2)` THEN1
   (FULL_SIMP_TAC std_ss [FLOOKUP_DEF, FAPPLY_FUPDATE_THM, FDOM_FUPDATE, IN_INSERT] THEN 
   RW_TAC bool_ss [] THEN FULL_SIMP_TAC bool_ss [] THEN METIS_TAC []) THEN
 FULL_SIMP_TAC std_ss [FLOOKUP_DEF, FAPPLY_FUPDATE_THM, FDOM_FUPDATE, IN_INSERT] THEN RW_TAC bool_ss [] THEN
-`map_line_admitted (G |+ (INL l1,INL p1)) /\ map_box_admitted (G |+ (INL l1,INL p1))` suffices_by METIS_TAC [map_box_admitted] THEN
+`map_line_admitted (G |+ (INL l1,INL p1)) a /\ map_box_admitted (G |+ (INL l1,INL p1)) a` suffices_by METIS_TAC [map_box_admitted] THEN
 CONJ_TAC THEN1
  (RW_TAC bool_ss [map_line_admitted] THEN
   Cases_on `l1 = l'` THEN FULL_SIMP_TAC std_ss [FLOOKUP_DEF, FAPPLY_FUPDATE_THM, FDOM_FUPDATE, IN_INSERT] THEN
@@ -341,9 +342,9 @@ RW_TAC bool_ss [FLOOKUP_DEF]
 QED
 
 Theorem soundness_proof_aux[local]:
- !G pl pr. valid_proof G pl pr ==> soundness_prop G pl pr
+ !G pl pr. valid_proof G pl pr ==> !a. soundness_prop G pl pr a
 Proof
-MATCH_MP_TAC valid_proof_ind >> RW_TAC list_ss [] >| [
+HO_MATCH_MP_TAC valid_proof_ind >> RW_TAC list_ss [] >| [
  PROVE_TAC [soundness_empty],
  PROVE_TAC [soundness_derivation],
  PROVE_TAC [soundness_box]
@@ -351,20 +352,20 @@ MATCH_MP_TAC valid_proof_ind >> RW_TAC list_ss [] >| [
 QED
 
 Theorem soundness_proof:
- !G pl pr p l j. premises_admitted pl ==>
-  map_line_admitted G ==>
-  map_box_admitted G ==>
+ !G pl pr p l j a. premises_admitted pl a ==>
+  map_line_admitted G a ==>
+  map_box_admitted G a ==>
   valid_proof G pl pr ==>
   MEM (entry_derivation (derivation_deriv l p (reason_justification j))) pr ==>
-  prop_of p
+  prop_sem p a
 Proof
  METIS_TAC [soundness_proof_aux,soundness_prop]
 QED
 
 Theorem soundness_claim:
- !p pl pr. premises_admitted pl ==>
+ !p pl pr a. premises_admitted pl a ==>
  valid_claim (claim_judgment_proof (judgment_follows pl p) pr) ==>
- prop_of p
+ prop_sem p a
 Proof
  SUBGOAL_THEN ``(!a0. valid_claim a0 <=>
   ?proplist prop proof l j. a0 = claim_judgment_proof (judgment_follows proplist prop) proof /\
@@ -373,9 +374,9 @@ Proof
    entry_derivation (derivation_deriv l prop (reason_justification j)) /\
   valid_proof FEMPTY proplist proof)`` ASSUME_TAC THEN1 METIS_TAC [valid_claim_cases] THEN
  RW_TAC list_ss [] THEN
- SUBGOAL_THEN ``map_line_admitted (FEMPTY:num + num # num |-> prop + prop # prop)`` ASSUME_TAC THEN1
+ SUBGOAL_THEN ``map_line_admitted (FEMPTY:num + num # num |-> prop + prop # prop) a`` ASSUME_TAC THEN1
  RW_TAC list_ss [map_line_admitted, FLOOKUP_DEF, FDOM_FEMPTY] THEN
- SUBGOAL_THEN ``map_box_admitted (FEMPTY:num + num # num |-> prop + prop # prop)`` ASSUME_TAC THEN1
+ SUBGOAL_THEN ``map_box_admitted (FEMPTY:num + num # num |-> prop + prop # prop) a`` ASSUME_TAC THEN1
  RW_TAC list_ss [map_box_admitted, FLOOKUP_DEF, FDOM_FEMPTY] THEN
 
  Cases_on `pr` THEN1
